{
 "cells": [
  {
   "cell_type": "code",
   "execution_count": null,
   "id": "d8ee98a5",
   "metadata": {},
   "outputs": [],
   "source": [
    "#1. Find the value of T(2) for the recurrence relation T(n) = 3T(n-1) + 12n, given that T(0)=5.\n",
    "\n",
    "Given:\n",
    "Recurrence relation: \n",
    "\n",
    "T(n) = 3T(n-1) + 12n\n",
    "T(0)=5\n",
    "\n",
    "T(1) = 3T(1-1) + 12*1\n",
    "T(1) = 3*T(0) + 12\n",
    "\n",
    "we have to find the value of T(2):\n",
    "    \n",
    "    T(2) = 3T(2-1) + 12*2\n",
    "    T(2) = 3*T(1) + 24\n",
    "    T(2) = 3(3*T(0) + 12) + 24 # substituting the value of T(1)\n",
    "    T(2) = 3(3*5 +12) + 24\n",
    "    T(2) = 105\n",
    "    \n",
    "The value of T(2) is 105\n"
   ]
  },
  {
   "cell_type": "code",
   "execution_count": null,
   "id": "75b3a80f",
   "metadata": {},
   "outputs": [],
   "source": [
    "2. Given a recurrence relation, solve it using the substitution method:\n",
    "a. T(n) = T(n-1) + c\n",
    "b. T(n) = 2T(n/2) + n\n",
    "c. T(n) = 2T(n/2) + c\n",
    "d. T(n) = T(n/2) + c\n",
    "\n",
    "\n",
    "# a. T(n) = T(n-1) + c\n",
    "# T(n) = T(n-1) + c = T(n-2) + c + c = T(n-3) + c + c + c = ... = T(n-k) + kc\n",
    "# Base case: T(0) = b\n",
    "\n",
    "# b. T(n) = 2T(n/2) + n\n",
    "# T(n) = 2T(n/2) + n = 2(2T(n/4) + n/2) + n = 2^2T(n/2^2) + 2n = 2^3T(n/2^3) + 3n = ... = 2^kT(n/2^k) + kn\n",
    "# Base case: T(1) = c\n",
    "\n",
    "# c. T(n) = 2T(n/2) + c\n",
    "# T(n) = 2T(n/2) + c = 2(2T(n/4) + c) + c = 2^2T(n/2^2) + 2c + c = 2^3T(n/2^3) + 4c + c = ... = 2^kT(n/2^k) + kc\n",
    "# Base case: T(1) = c\n",
    "\n",
    "# d. T(n) = T(n/2) + c\n",
    "# T(n) = T(n/2) + c = T(n/4) + c + c = T(n/8) + c + c + c = ... = T(1) + log(n) * c\n",
    "# Base case: T(1) = c\n",
    "\n"
   ]
  },
  {
   "cell_type": "code",
   "execution_count": null,
   "id": "b3a68dc8",
   "metadata": {},
   "outputs": [],
   "source": [
    "3. Given a recurrence relation, solve it using the recursive tree approach:\n",
    "a. T(n) = 2T(n-1) +1\n",
    "T(n) = 2T(n-1) + 1\n",
    "     = 2[2T(n-2) + 1] + 1\n",
    "     = 2^2T(n-2) + 2 + 1\n",
    "     = 2^3T(n-3) + 2^2 + 2 + 1\n",
    "     ...\n",
    "     = 2^kT(n-k) + 2^k - 1 + ... + 2^2 + 2 + 1\n",
    "\n",
    "When n - k = 1 (base case),\n",
    "T(1) = 2T(0) + 1 (assuming T(0) = 1 or any base case value)\n",
    "\n",
    "If we substitute k = n - 1, we get:\n",
    "T(n) = 2^nT(1) + 2^n - 1 + 2^(n-1) + ... + 2^2 + 2 + 1\n",
    "     = 2^n * T(1) + (2^n - 1) + (2^n - 2) + ... + 2 + 1\n",
    "     = 2^n * T(1) + (2^n - 1) * 2 / 1 (sum of first n terms of a geometric series)\n",
    "     = 2^n * T(1) + 2^(n+1) - 2 - 2\n",
    "     = 2^n * T(1) + 2^(n+1) - 4\n",
    "\n",
    "        \n",
    "        \n",
    "b. T(n) = 2T(n/2) + n\n",
    "T(n) = 2T(n/2) + n\n",
    "     = 2[2T(n/4) + n/2] + n\n",
    "     = 2^2T(n/4) + 2n/2 + n\n",
    "     = 2^2T(n/4) + 3n/2\n",
    "     ...\n",
    "     = 2^kT(n/2^k) + kn/(2^(k-1))\n",
    "\n",
    "When n/2^k = 1 (base case),\n",
    "n = 2^k\n",
    "k = log2(n)\n",
    "\n",
    "T(1) = 1 (assuming T(1) = 1 or any base case value)\n",
    "\n",
    "If we substitute k = log2(n), we get:\n",
    "T(n) = 2^(log2(n)) * T(1) + n * log2(n)\n",
    "     = n * T(1) + n * log2(n)\n",
    "\n"
   ]
  }
 ],
 "metadata": {
  "kernelspec": {
   "display_name": "Python 3 (ipykernel)",
   "language": "python",
   "name": "python3"
  },
  "language_info": {
   "codemirror_mode": {
    "name": "ipython",
    "version": 3
   },
   "file_extension": ".py",
   "mimetype": "text/x-python",
   "name": "python",
   "nbconvert_exporter": "python",
   "pygments_lexer": "ipython3",
   "version": "3.11.4"
  }
 },
 "nbformat": 4,
 "nbformat_minor": 5
}
